sir/Sir/Vars/Proofs/Quotient.lean
@@ -2,24 +2,24 @@ import Sir.Vars.Spec.Quotient
 
 namespace Sir.Vars.Proofs
 
-private def canonicalProgramEquivalenceClass :
-    { program : Program // program.Canonical } → Quotient Program.alphaEquivalenceSetoid :=
+private def normalProgramEquivalenceClass :
+    { program : Program // program.Normal } → Quotient Program.alphaEquivalenceSetoid :=
   fun program => Quotient.mk Program.alphaEquivalenceSetoid program
 
-private theorem canonicalProgramEquivalenceClass_leftInverse :
-    Function.LeftInverse canonicalProgramEquivalenceClass
-      Program.canonicalizeEquivalenceClass := by
+private theorem normalProgramEquivalenceClass_leftInverse :
+    Function.LeftInverse normalProgramEquivalenceClass
+      Program.normalizeEquivalenceClass := by
   intro equivalenceClass
   refine Quotient.inductionOn equivalenceClass ?_
   intro program
-  exact Quotient.sound (Program.canonicalize_alphaEquiv program)
+  exact Quotient.sound (Program.normalize_alphaEquiv program)
 
-theorem Program.canonicalizeEquivalenceClass_bijective :
-    Function.Bijective Vars.Program.canonicalizeEquivalenceClass := by
+theorem Program.normalizeEquivalenceClass_bijective :
+    Function.Bijective Vars.Program.normalizeEquivalenceClass := by
   constructor
-  · exact canonicalProgramEquivalenceClass_leftInverse.injective
+  · exact normalProgramEquivalenceClass_leftInverse.injective
   · intro program
-    refine ⟨canonicalProgramEquivalenceClass program, ?_⟩
+    refine ⟨normalProgramEquivalenceClass program, ?_⟩
     exact Subtype.ext program.property
 
 end Sir.Vars.Proofs
